Add spatial_graph definitions.

data_structure/spatial_graph.v
@@ -1,10 +1,16 @@
 Require Import VST.msl.seplog.
 Require Import RamifyCoq.msl_ext.abs_addr.
 Require Import RamifyCoq.msl_ext.seplog.
+Require Import RamifyCoq.msl_ext.log_normalize.
+Require Import RamifyCoq.msl_ext.iter_sepcon.
+Require Import RamifyCoq.graph.graph.
+Require Import RamifyCoq.graph.graph_reachable.
+Import RamifyCoq.msl_ext.seplog.OconNotation.
 
 Class SpatialGraphSetting: Type := {
   Data: Type;
   addr: Type;
+  null: addr;
   addr_eq_dec: forall x y: addr, {x = y} + {x <> y};
   addr_eqb: addr -> addr -> bool := fun x y => if addr_eq_dec x y then true else false
 }.
@@ -16,6 +22,8 @@ Instance AV_SGraph `{SpatialGraphSetting} : AbsAddr.
   + unfold addr_eqb in H0.
     destruct (addr_eq_dec p1 p1); congruence.
 Defined.
+
+Instance AddrDec `{SpatialGraphSetting}: EqDec Addr. apply Build_EqDec. intros. apply (addr_eq_dec t1 t2). Defined.
 
 Class SpatialGraphAssum: Type := {
   SGA_Pred: Type;
@@ -40,11 +48,35 @@ Hint Resolve SGA_ND SGA_SL SGA_ClSL SGA_PSL SGA_CoSL SGA_OSL SGA_DSL SG_Setting 
 
 Local Open Scope logic.
 
-Lemma foo: forall `{SpatialGraphAssum} p v, trinode p v * trinode p v |-- FF.
-Proof.
-  intros.
-  apply mapsto_conflict.
-  simpl.
-  unfold addr_eqb.
-  destruct addr_eq_dec; congruence.
-Qed.
+Section SpatialGraph.
+
+  Context {SGA : SpatialGraphAssum}.
+
+  Definition graph_cell (bi : BiGraph Addr Data) (v : Addr) : SGA_Pred := trinode v (gamma bi v).
+
+  Lemma precise_graph_cell: forall bi v, precise (graph_cell bi v).
+  Proof. intros. unfold graph_cell. destruct (gamma bi v) as [[? ?] ?]. apply mapsto_precise. Qed.
+
+  Lemma sepcon_unique_graph_cell: forall bi, sepcon_unique (graph_cell bi).
+  Proof.
+    repeat intro. unfold graph_cell. destruct (gamma bi x) as [[? ?] ?]. apply mapsto_conflict.
+    simpl. unfold addr_eqb. destruct (addr_eq_dec x x); auto.
+  Qed.
+
+  Definition graph (x : Addr) (bimg : BiMathGraph Addr Data null): SGA_Pred :=
+    (!!(x = null) && emp) || EX l : list Addr, !!reachable_list b_pg x l && iter_sepcon l (graph_cell bm_bi).
+
+  Lemma graph_unfold:
+    forall x bimg,
+      graph x bimg = (!!(x = null) && emp) ||
+                     EX d:Data, EX l:Addr, EX r:Addr, !!(gamma bm_bi x = (d, l, r) /\ valid x) &&
+                                                        (trinode x (d, l, r) ⊗ graph l bimg ⊗ graph r bimg).
+  Proof.
+    intros. apply pred_ext.
+    + unfold graph at 1. apply orp_left.
+      - apply orp_right1. apply derives_refl.
+      - apply orp_right2. apply exp_left; intro l.
+        destruct (gamma bm_bi x) as [[dd ll] rr]. apply (exp_right dd), (exp_right ll), (exp_right rr).
+  Abort.
+
+End SpatialGraph.
